rustfrontend/Rusttyping.v
@@ -158,6 +158,10 @@ Inductive variance :=
 | Covariant
 | Invariant.
 
+Lemma variance_eq: forall (va1 va2: variance), {va1 = va2} + {va1 <> va2}.
+decide equality.
+Defined.
+
 Definition join_variance (v1 v2: variance) :=
   match v1, v2 with
   | Invariant, _
